@prefix : <http://streamreasoning.org/vois#> .
@prefix sd: <http://www.w3.org/ns/sparql-service-description#> .
@prefix owl: <http://www.w3.org/2002/07/owl#> .
@prefix rdf: <http://www.w3.org/1999/02/22-rdf-syntax-ns#> .
@prefix xml: <http://www.w3.org/XML/1998/namespace> .
@prefix xsd: <http://www.w3.org/2001/XMLSchema#> .
@prefix frmt: <http://www.w3.org/ns/formats/> .
@prefix rdfs: <http://www.w3.org/2000/01/rdf-schema#> .
@prefix time: <http://www.w3.org/2006/time#> .
@prefix vois: <http://streamreasoning.org/vois#> .
@base <http://streamreasoning.org/vois> .

<http://streamreasoning.org/vois> rdf:type owl:Ontology ;
                                   owl:versionIRI <http://streamreasoning.org/vois/2.0.0> .

#################################################################
#    Annotation properties
#################################################################

###  http://www.w3.org/ns/sparql-service-description#name
sd:name rdf:type owl:AnnotationProperty ;
        rdfs:comment "Relates a named graph to the name by which it may be referenced in a FROM/FROM NAMED clause. The object of the sd:name property is an IRI." ;
        rdfs:label "name" ;
        rdfs:domain sd:NamedGraph .


#################################################################
#    Object Properties
#################################################################

###  http://streamreasoning.org/vois#availableGraphs
vois:availableGraphs rdf:type owl:ObjectProperty ;
                     rdfs:subPropertyOf owl:topObjectProperty ;
                     rdfs:domain vois:RSPService ;
                     rdfs:range vois:Window .


###  http://streamreasoning.org/vois#defaultGraph
vois:defaultGraph rdf:type owl:ObjectProperty ;
                  rdfs:domain vois:RDFStream ;
                  rdfs:range sd:Graph ;
                  rdfs:comment "Relates an instance of vois:RDFStream to the description of its default graph." .


###  http://streamreasoning.org/vois#endedAt
vois:endedAt rdf:type owl:ObjectProperty ;
             rdfs:subPropertyOf owl:topObjectProperty ;
             rdfs:domain vois:Window ;
             rdfs:range time:Instant .


###  http://streamreasoning.org/vois#graph
vois:graph rdf:type owl:ObjectProperty ;
           rdfs:subPropertyOf owl:topObjectProperty ;
           rdfs:domain sd:NamedGraph ;
           rdfs:range sd:Graph ;
           rdfs:comment "Relates a named graph to its graph description." .


###  http://streamreasoning.org/vois#namedGraph
vois:namedGraph rdf:type owl:ObjectProperty ;
                rdfs:subPropertyOf owl:topObjectProperty ;
                rdfs:domain vois:Window ;
                rdfs:range sd:NamedGraph ;
                rdfs:comment "Relates an instance of vois:Window to the description of one of its named graphs. The description of such a named graph MUST include the sd:name property." ;
                rdfs:label "named graph" .


###  http://streamreasoning.org/vois#resultFormat
vois:resultFormat rdf:type owl:ObjectProperty ;
                  rdfs:domain vois:RSPService ;
                  rdfs:range frmt:Format ;
                  rdfs:comment "Relates an instance of sd:Service to a format that is supported for serializing query results." ;
                  rdfs:label "result format" .


###  http://streamreasoning.org/vois#rspEndpoint
vois:rspEndpoint rdf:type owl:ObjectProperty ;
                 rdfs:subPropertyOf owl:topObjectProperty ;
                 rdfs:domain vois:RSPService ;
                 rdfs:comment "The RSP-QL endpoint of an vois:RSPService that implements the RSP-QL Protocol service. The object of the vois:rspEndpoint property is an IRI." ;
                 rdfs:label "RSP endpoint" .


###  http://streamreasoning.org/vois#startedAt
vois:startedAt rdf:type owl:ObjectProperty ;
               rdfs:subPropertyOf owl:topObjectProperty ;
               rdfs:domain vois:Window ;
               rdfs:range time:Instant .


###  http://streamreasoning.org/vois#startingTime
vois:startingTime rdf:type owl:ObjectProperty ;
                  rdfs:subPropertyOf owl:topObjectProperty ;
                  rdfs:domain vois:WindowOperator ;
                  rdfs:range time:Instant .


###  http://www.w3.org/ns/sparql-service-description#availableGraphs
sd:availableGraphs rdf:type owl:ObjectProperty ;
                   rdfs:domain sd:Service ;
                   rdfs:range sd:GraphCollection ;
                   rdfs:comment "Relates an instance of sd:Service to a description of the graphs which are allowed in the construction of a dataset either via the SPARQL Protocol, with FROM/FROM NAMED clauses in a query, or with USING/USING NAMED in an update request, if the service limits the scope of dataset construction." ;
                   rdfs:label "available graph descriptions" .


###  http://www.w3.org/ns/sparql-service-description#defaultDataset
sd:defaultDataset rdf:type owl:ObjectProperty ,
                           owl:InverseFunctionalProperty ;
                  rdfs:domain sd:Service ;
                  rdfs:range sd:Dataset ;
                  rdfs:comment "Relates an instance of sd:Service to a description of the default dataset available when no explicit dataset is specified in the query, update request or via protocol parameters." ;
                  rdfs:label "default dataset description" .


###  http://www.w3.org/ns/sparql-service-description#defaultEntailmentRegime
sd:defaultEntailmentRegime rdf:type owl:ObjectProperty ;
                           rdfs:subPropertyOf sd:feature ;
                           rdfs:domain sd:Service ;
                           rdfs:range sd:EntailmentRegime ;
                           rdfs:comment "Relates an instance of sd:Service with a resource representing an entailment regime used for basic graph pattern matching. This property is intended for use when a single entailment regime by default applies to all graphs in the default dataset of the service. In situations where a different entailment regime applies to a specific graph in the dataset, the sd:entailmentRegime property should be used to indicate this fact in the description of that graph." ;
                           rdfs:label "default entailment regime" .


###  http://www.w3.org/ns/sparql-service-description#defaultGraph
sd:defaultGraph rdf:type owl:ObjectProperty ;
                rdfs:domain sd:Dataset ;
                rdfs:range sd:Graph ;
                rdfs:comment "Relates an instance of sd:Dataset to the description of its default graph." ;
                rdfs:label "default graph" .


###  http://www.w3.org/ns/sparql-service-description#defaultSupportedEntailmentProfile
sd:defaultSupportedEntailmentProfile rdf:type owl:ObjectProperty ;
                                     rdfs:subPropertyOf sd:feature ;
                                     rdfs:domain sd:Service ;
                                     rdfs:range sd:EntailmentProfile ;
                                     rdfs:comment "Relates an instance of sd:Service with a resource representing a supported profile of the default entailment regime (as declared by sd:defaultEntailmentRegime)." ;
                                     rdfs:label "default supported entailment profile" .


###  http://www.w3.org/ns/sparql-service-description#endpoint
sd:endpoint rdf:type owl:ObjectProperty ,
                     owl:InverseFunctionalProperty ;
            rdfs:domain sd:Service ;
            rdfs:comment "The SPARQL endpoint of an sd:Service that implements the SPARQL Protocol service. The object of the sd:endpoint property is an IRI." ;
            rdfs:label "endpoint" .


###  http://www.w3.org/ns/sparql-service-description#extensionAggregate
sd:extensionAggregate rdf:type owl:ObjectProperty ;
                      rdfs:subPropertyOf sd:feature ;
                      rdfs:domain sd:Service ;
                      rdfs:range sd:Aggregate ;
                      rdfs:comment "Relates an instance of sd:Service to an aggregate that may be used in a SPARQL aggregate query (for instance in a HAVING clause or SELECT expression) besides the standard list of supported aggregates COUNT, SUM, MIN, MAX, AVG, GROUP_CONCAT, and SAMPLE" ;
                      rdfs:label "extension aggregate" .


###  http://www.w3.org/ns/sparql-service-description#extensionFunction
sd:extensionFunction rdf:type owl:ObjectProperty ;
                     rdfs:subPropertyOf sd:feature ;
                     rdfs:domain sd:Service ;
                     rdfs:range sd:Function ;
                     rdfs:comment "Relates an instance of sd:Service to a function that may be used in a SPARQL SELECT expression or a FILTER, HAVING, GROUP BY, ORDER BY, or BIND clause." ;
                     rdfs:label "extension function" .


###  http://www.w3.org/ns/sparql-service-description#feature
sd:feature rdf:type owl:ObjectProperty ;
           rdfs:domain sd:Service ;
           rdfs:range sd:Feature ;
           rdfs:comment "Relates an instance of sd:Service with a resource representing a supported feature." ;
           rdfs:label "feature" .


###  http://www.w3.org/ns/sparql-service-description#graph
sd:graph rdf:type owl:ObjectProperty ;
         rdfs:domain sd:NamedGraph ;
         rdfs:range sd:Graph ;
         rdfs:comment "Relates a named graph to its graph description." ;
         rdfs:label "graph" .


###  http://www.w3.org/ns/sparql-service-description#inputFormat
sd:inputFormat rdf:type owl:ObjectProperty ;
               rdfs:domain sd:Service ;
               rdfs:range frmt:Format ;
               rdfs:comment "Relates an instance of sd:Service to a format that is supported for parsing RDF input; for example, via a SPARQL 1.1 Update LOAD statement, or when URIs are dereferenced in FROM/FROM NAMED/USING/USING NAMED clauses." ;
               rdfs:label "input format" .


###  http://www.w3.org/ns/sparql-service-description#languageExtension
sd:languageExtension rdf:type owl:ObjectProperty ;
                     rdfs:subPropertyOf sd:feature ;
                     rdfs:domain sd:Service ;
                     rdfs:range sd:Feature ;
                     rdfs:comment "Relates an instance of sd:Service to a resource representing an implemented extension to the SPARQL Query or Update language." ;
                     rdfs:label "language extension" .


###  http://www.w3.org/ns/sparql-service-description#namedGraph
sd:namedGraph rdf:type owl:ObjectProperty ;
              rdfs:domain sd:GraphCollection ;
              rdfs:range sd:NamedGraph ;
              rdfs:comment "Relates an instance of sd:GraphCollection (or its subclass sd:Dataset) to the description of one of its named graphs. The description of such a named graph MUST include the sd:name property and MAY include the sd:graph property." ;
              rdfs:label "named graph" .


###  http://www.w3.org/ns/sparql-service-description#propertyFeature
sd:propertyFeature rdf:type owl:ObjectProperty ;
                   rdfs:subPropertyOf sd:feature ;
                   rdfs:domain sd:Service ;
                   rdfs:range sd:Feature ;
                   rdfs:comment "Relates an instance of sd:Service to a resource representing an implemented feature that extends the SPARQL Query or Update language and that is accessed by using the named property." ;
                   rdfs:label "property feature" .


###  http://www.w3.org/ns/sparql-service-description#resultFormat
sd:resultFormat rdf:type owl:ObjectProperty ;
                rdfs:domain sd:Service ;
                rdfs:range frmt:Format ;
                rdfs:comment "Relates an instance of sd:Service to a format that is supported for serializing query results." ;
                rdfs:label "result format" .


###  http://www.w3.org/ns/sparql-service-description#supportedLanguage
sd:supportedLanguage rdf:type owl:ObjectProperty ;
                     rdfs:subPropertyOf sd:feature ;
                     rdfs:domain sd:Service ;
                     rdfs:range sd:Language ;
                     rdfs:comment "Relates an instance of sd:Service to a SPARQL language (e.g. Query and Update) that it implements." ;
                     rdfs:label "supported language" .


#################################################################
#    Data properties
#################################################################

###  http://streamreasoning.org/vois#range
vois:range rdf:type owl:DatatypeProperty ;
           rdfs:domain vois:WindowOperator ;
           rdfs:range xsd:positiveInteger .


###  http://streamreasoning.org/vois#step
vois:step rdf:type owl:DatatypeProperty ;
          rdfs:domain vois:WindowOperator ;
          rdfs:range xsd:positiveInteger .


#################################################################
#    Classes
#################################################################

###  http://streamreasoning.org/vois#PhysicalWindow
vois:PhysicalWindow rdf:type owl:Class ;
                    rdfs:subClassOf vois:Window ;
                    rdfs:comment "Window defined by an interval size (in units of RDF elements)" .


###  http://streamreasoning.org/vois#PhysicalWindowOperator
vois:PhysicalWindowOperator rdf:type owl:Class ;
                            rdfs:subClassOf vois:WindowOperator ;
                            owl:disjointWith vois:TimeBasedWindowOperator ;
                            rdfs:comment "Operator sampling the data stream into PhysicalWindow, i.e. based on the size of the window not a time interval" .


###  http://streamreasoning.org/vois#RDFStream
vois:RDFStream rdf:type owl:Class ;
               rdfs:comment "A stream composed of non decreasing timestamped RDF data elements, i.e. RDF graphs and/or triples." ;
               rdfs:label "RDFStream" .


###  http://streamreasoning.org/vois#RSPService
vois:RSPService rdf:type owl:Class ;
                rdfs:comment "An instance of vois:Service represents a RSP service made available via the RSP Protocol." .


###  http://streamreasoning.org/vois#StreamingDataset
vois:StreamingDataset rdf:type owl:Class ;
                      rdfs:comment "A streaming dataset is a set composed by an (optional) default graph, n (n ≥ 0) named graphs and m (m ≥ 0) named time-varying graphs" ;
                      rdfs:label "SDS" .


###  http://streamreasoning.org/vois#TimeBasedWindow
vois:TimeBasedWindow rdf:type owl:Class ;
                     rdfs:subClassOf vois:Window ;
                     rdfs:comment "A time-based window is a window defined through two time instants o, c (respectively named opening and closing time instants) such that: W(S) = {d|(d, t) ∈ S ∧ t ∈ (o, c]}" .


###  http://streamreasoning.org/vois#TimeBasedWindowOperator
vois:TimeBasedWindowOperator rdf:type owl:Class ;
                             rdfs:subClassOf vois:WindowOperator ;
                             rdfs:comment "Operator sampling the data stream into TimeBasedWindow, i.e. based on time intervals not the size of the window" .


###  http://streamreasoning.org/vois#TimeVarryingGraph
vois:TimeVarryingGraph rdf:type owl:Class ;
                       rdfs:comment "A time-varying graph G is a function that relates time instants t ∈ T to RDF graphs: G : T → {g | g is an RDF graph}" .


###  http://streamreasoning.org/vois#Window
vois:Window rdf:type owl:Class ;
            rdfs:subClassOf <http://www.w3.org/ns/dcat#Dataset> ;
            rdfs:comment "A window W(S) is a set of RDF statements extracted from a stream S." .


###  http://streamreasoning.org/vois#WindowOperator
vois:WindowOperator rdf:type owl:Class ;
                    rdfs:subClassOf <http://www.w3.org/ns/prov#Activity> ;
                    rdfs:comment "Operator that sample the data stream to window" .


###  http://www.w3.org/2006/time#Instant
time:Instant rdf:type owl:Class .


###  http://www.w3.org/ns/dcat#Dataset
<http://www.w3.org/ns/dcat#Dataset> rdf:type owl:Class .


###  http://www.w3.org/ns/formats/Format
frmt:Format rdf:type owl:Class .


###  http://www.w3.org/ns/prov#Activity
<http://www.w3.org/ns/prov#Activity> rdf:type owl:Class .


###  http://www.w3.org/ns/sparql-service-description#Aggregate
sd:Aggregate rdf:type owl:Class ;
             rdfs:subClassOf sd:Feature ;
             rdfs:comment "An instance of sd:Aggregate represents an aggregate that may be used in a SPARQL aggregate query (for instance in a HAVING clause or SELECT expression) besides the standard list of supported aggregates COUNT, SUM, MIN, MAX, AVG, GROUP_CONCAT, and SAMPLE." ;
             rdfs:label "Aggregate" .


###  http://www.w3.org/ns/sparql-service-description#Dataset
sd:Dataset rdf:type owl:Class ;
           rdfs:subClassOf sd:GraphCollection ;
           rdfs:comment "An instance of sd:Dataset represents a RDF Dataset comprised of a default graph and zero or more named graphs." ;
           rdfs:label "Dataset" .


###  http://www.w3.org/ns/sparql-service-description#EntailmentProfile
sd:EntailmentProfile rdf:type owl:Class ;
                     rdfs:subClassOf sd:Feature ;
                     rdfs:comment "An instance of sd:EntailmentProfile represents a profile of an entailment regime. An entailment profile MAY impose restrictions on what constitutes valid RDF with respect to entailment." ;
                     rdfs:label "Entailment Profile" .


###  http://www.w3.org/ns/sparql-service-description#EntailmentRegime
sd:EntailmentRegime rdf:type owl:Class ;
                    rdfs:subClassOf sd:Feature ;
                    rdfs:comment "An instance of sd:EntailmentRegime represents an entailment regime used in basic graph pattern matching (as described by SPARQL 1.1 Query Language)." ;
                    rdfs:label "Entailment Regime" .


###  http://www.w3.org/ns/sparql-service-description#Feature
sd:Feature rdf:type owl:Class ;
           rdfs:comment "An instance of sd:Feature represents a feature of a SPARQL service. Specific types of features include functions, aggregates, languages, and entailment regimes and profiles. This document defines five instances of sd:Feature: sd:DereferencesURIs, sd:UnionDefaultGraph, sd:RequiresDataset, sd:EmptyGraphs, and sd:BasicFederatedQuery." ;
           rdfs:label "Feature" .


###  http://www.w3.org/ns/sparql-service-description#Function
sd:Function rdf:type owl:Class ;
            rdfs:subClassOf sd:Feature ;
            rdfs:comment "An instance of sd:Function represents a function that may be used in a SPARQL SELECT expression or a FILTER, HAVING, GROUP BY, ORDER BY, or BIND clause." ;
            rdfs:label "Function" .


###  http://www.w3.org/ns/sparql-service-description#Graph
sd:Graph rdf:type owl:Class ;
         rdfs:comment "An instance of sd:Graph represents the description of an RDF graph." ;
         rdfs:label "Graph" .


###  http://www.w3.org/ns/sparql-service-description#GraphCollection
sd:GraphCollection rdf:type owl:Class ;
                   rdfs:comment "An instance of sd:GraphCollection represents a collection of zero or more named graph descriptions. Each named graph description belonging to an sd:GraphCollection MUST be linked with the sd:namedGraph predicate." ;
                   rdfs:label "Graph Collection" .


###  http://www.w3.org/ns/sparql-service-description#Language
sd:Language rdf:type owl:Class ;
            rdfs:subClassOf sd:Feature ;
            rdfs:comment "An instance of sd:Language represents one of the SPARQL languages, including specific configurations providing particular features or extensions. This document defines three instances of sd:Language: sd:SPARQL10Query, sd:SPARQL11Query, and sd:SPARQL11Update." ;
            rdfs:label "Language" .


###  http://www.w3.org/ns/sparql-service-description#NamedGraph
sd:NamedGraph rdf:type owl:Class ;
              rdfs:comment "An instance of sd:NamedGraph represents a named graph having a name (via sd:name) and an optional graph description (via sd:graph)." ;
              rdfs:label "Named Graph" .


###  http://www.w3.org/ns/sparql-service-description#Service
sd:Service rdf:type owl:Class ;
           rdfs:comment "An instance of sd:Service represents a SPARQL service made available via the SPARQL Protocol." ;
           rdfs:label "Service" .


#################################################################
#    Individuals
#################################################################

###  http://www.w3.org/ns/sparql-service-description#BasicFederatedQuery
sd:BasicFederatedQuery rdf:type owl:NamedIndividual ,
                                sd:Feature ;
                       rdfs:comment "sd:BasicFederatedQuery, when used as the object of the sd:feature property, indicates that the SPARQL service supports basic federated query using the SERVICE keyword as defined by SPARQL 1.1 Federation Extensions." ;
                       rdfs:label "Basic Federated Query" .


###  http://www.w3.org/ns/sparql-service-description#DereferencesURIs
sd:DereferencesURIs rdf:type owl:NamedIndividual ,
                             sd:Feature ;
                    rdfs:comment "sd:DereferencesURIs, when used as the object of the sd:feature property, indicates that a SPARQL service will dereference URIs used in FROM/FROM NAMED and USING/USING NAMED clauses and use the resulting RDF in the dataset during query evaluation." ;
                    rdfs:label "Dereferences URIs" .


###  http://www.w3.org/ns/sparql-service-description#EmptyGraphs
sd:EmptyGraphs rdf:type owl:NamedIndividual ,
                        sd:Feature ;
               rdfs:comment "sd:EmptyGraphs, when used as the object of the sd:feature property, indicates that the underlying graph store supports empty graphs. A graph store that supports empty graphs MUST NOT remove graphs that are left empty after triples are removed from them." ;
               rdfs:label "Empty Graphs" .


###  http://www.w3.org/ns/sparql-service-description#RequiresDataset
sd:RequiresDataset rdf:type owl:NamedIndividual ,
                            sd:Feature ;
                   rdfs:comment "sd:RequiresDataset, when used as the object of the sd:feature property, indicates that the SPARQL service requires an explicit dataset declaration (based on either FROM/FROM NAMED clauses in a query, USING/USING NAMED clauses in an update, or the appropriate SPARQL Protocol parameters)." ;
                   rdfs:label "Requires Dataset" .


###  http://www.w3.org/ns/sparql-service-description#SPARQL10Query
sd:SPARQL10Query rdf:type owl:NamedIndividual ,
                          sd:Language ;
                 rdfs:comment "sd:SPARQL10Query is an sd:Language representing the SPARQL 1.0 Query language." ;
                 rdfs:label "SPARQL 1.0 Query" .


###  http://www.w3.org/ns/sparql-service-description#SPARQL11Query
sd:SPARQL11Query rdf:type owl:NamedIndividual ,
                          sd:Language ;
                 rdfs:comment "sd:SPARQL11Query is an sd:Language representing the SPARQL 1.1 Query language." ;
                 rdfs:label "SPARQL 1.1 Query" .


###  http://www.w3.org/ns/sparql-service-description#SPARQL11Update
sd:SPARQL11Update rdf:type owl:NamedIndividual ,
                           sd:Language ;
                  rdfs:comment "sd:SPARQLUpdate is an sd:Language representing the SPARQL 1.1 Update language." ;
                  rdfs:label "SPARQL 1.1 Update" .


###  http://www.w3.org/ns/sparql-service-description#UnionDefaultGraph
sd:UnionDefaultGraph rdf:type owl:NamedIndividual ,
                              sd:Feature ;
                     rdfs:comment "sd:UnionDefaultGraph, when used as the object of the sd:feature property, indicates that the default graph of the dataset used during query and update evaluation (when an explicit dataset is not specified) is comprised of the union of all the named graphs in that dataset." ;
                     rdfs:label "Union Default Graph" .


###  Generated by the OWL API (version 4.2.8.20170104-2310) https://github.com/owlcs/owlapi
